src/Model.PNE.fsti
@@ -1,14 +1,17 @@
 module Model.PNE
 
-open FStar.HyperStack
-
-open Mem
-
 module B = LowStar.Buffer
 module HS = FStar.HyperStack
 module I = Model.Indexing
 module U32 = FStar.UInt32
 module U128 = FStar.UInt128
+module Spec = Spec.Agile.Cipher
+
+#set-options "--fuel 0 --ifuel 0"
+
+open FStar.HyperStack
+open Mem
+open Model.Helpers
 
 /// Abbreviations for idealization
 /// ------------------------------
@@ -24,30 +27,40 @@ type safe_id =
 type unsafe_id =
   i:id{not (is_safe i)}
 
-let samplelen = 16
-type sample = lbytes samplelen
-type pne_plainlen = l:nat {l >= 2 /\ l <= 5}
-type pne_cipher (l:pne_plainlen) = lbytes l
-type pne_cipherpad = lbytes 5
+/// QUIC packet sampling
+/// --------------------
 
-val clip_cipherpad : (cp:pne_cipherpad) -> (l:pne_plainlen) -> pne_cipher l
+let sample_length = 16
+let sample = lbytes sample_length
+let pne_plain_length = l:nat {l >= 2 /\ l <= 5}
+let pne_cipher (l:pne_plain_length) = lbytes l
+let pne_cipherpad = lbytes 5
 
+/// Restrict a generated cipherpad to the length of the encoded packet number.
+val clip_cipherpad : (cp:pne_cipherpad) -> (l:pne_plain_length) -> pne_cipher l
+
+// We have to locally redefine the plain package since the one in AEAD has a
+// notion of minimum length, and a maximum length related to Spec.Agile.AEAD. We
+// could conceivably share definitions via some added type parameters or
+// refinements.
 noeq type pne_plain_pkg =
   | PNEPlainPkg:
-    pne_plain: (j:id -> l:pne_plainlen -> (t:Type0{hasEq t})) ->
-    as_bytes: (j:id -> l:pne_plainlen -> pne_plain j l -> GTot (lbytes l)) ->
-    repr: (j:unsafeid -> l:pne_plainlen -> n:pne_plain j l -> Tot (b:lbytes l{b == as_bytes j l n})) ->
+    pne_plain: (j:id -> l:pne_plain_length -> (t:Type0{hasEq t})) ->
+    as_bytes: (j:id -> l:pne_plain_length -> pne_plain j l -> GTot (lbytes l)) ->
+    repr: (j:unsafe_id -> l:pne_plain_length -> n:pne_plain j l -> Tot (b:lbytes l{b == as_bytes j l n})) ->
     pne_plain_pkg
 
+// JP: not sure why we don't have the same mechanism as for Model.AEAD with the index for `info`
 let info = pne_plain_pkg
 
-let pne_plain (u:info) (j:id) (l:pne_plainlen) =
+let pne_plain (u:info) (j:id) (l:pne_plain_length) =
   PNEPlainPkg?.pne_plain u j l
 
+noeq
 type entry (j:id) (u:info) =
   | Entry :
     s:sample ->
-    #l:pne_plainlen ->
+    #l:pne_plain_length ->
     n:pne_plain u j l ->
     c:pne_cipher l ->
     entry j u
@@ -56,19 +69,28 @@ val pne_state : (j:id) -> (u:info) -> Type0
 
 val table : (#j:id) -> (#u:info) -> (st:pne_state j u) -> (h:mem) -> GTot (Seq.seq (entry j u))
 
-val footprint : #j:id -> #u:info -> st:pne_state j u -> M.loc
+val footprint : #j:id -> #u:info -> st:pne_state j u -> B.loc
 
-val frame_table: #j:safeid -> #u:info -> st:pne_state j u -> l:Seq.seq (entry j u) ->
-  h0:mem -> r:M.loc -> h1:mem ->
+val invariant: #j:id -> #u:info -> st:pne_state j u -> mem -> Type0
+
+val frame_invariant: #j:id -> #u:info -> st:pne_state j u -> l:B.loc -> h0:mem -> h1:mem -> Lemma
+  (requires (
+    invariant st h0 /\
+    B.modifies l h0 h1 /\
+    B.loc_disjoint l (footprint st)))
+  (ensures (
+    invariant st h1))
+
+val frame_table: #j:safe_id -> #u:info -> st:pne_state j u ->
+  r:B.loc -> h0:mem -> h1:mem ->
   Lemma
     (requires
-      table st h0 == l /\
-      M.modifies r h0 h1 /\
-      r `M.loc_disjoint` (footprint st))
-    (ensures table st h1 == l)
+      B.modifies r h0 h1 /\
+      r `B.loc_disjoint` (footprint st))
+    (ensures table st h1 == table st h0)
 
 let sample_filter (j:id) (u:info) (s:sample) (e:entry j u) : bool =
-  Entry?.s e = s
+  Entry?.s e `lbytes_eq` s
 
 let entry_for_sample (#j:id) (#u:info) (s:sample) (st:pne_state j u) (h:mem) :
   GTot (option (entry j u)) =
@@ -82,19 +104,19 @@ let find_sample (#j:id) (#u:info) (s:sample) (st:pne_state j u) (h:mem) :
   GTot bool =
   Some? (entry_for_sample s st h)
 
-let sample_cipher_filter (j:id) (u:info) (s:sample) (#l:pne_plainlen) (c:pne_cipher l) (e:entry j u) : bool =
-  Entry?.s e = s && Entry?.l e = l && Entry?.c e = c
+let sample_cipher_filter (j:id) (u:info) (s:sample) (#l:pne_plain_length) (c:pne_cipher l) (e:entry j u) : bool =
+  Entry?.s e `lbytes_eq` s && Entry?.l e = l && Entry?.c e `lbytes_eq` c
 
-let entry_for_sample_cipher (#j:id) (#u:info) (s:sample) (#l:pne_plainlen) (c:pne_cipher l) (st:pne_state j u) (h:mem) :
+let entry_for_sample_cipher (#j:id) (#u:info) (s:sample) (#l:pne_plain_length) (c:pne_cipher l) (st:pne_state j u) (h:mem) :
   GTot (option (entry j u)) =
   Seq.find_l (sample_cipher_filter j u s #l c) (table st h)
 
-let find_sample_cipher (#j:id) (#u:info) (s:sample) (#l:pne_plainlen) (c:pne_cipher l) (st:pne_state j u) (h:mem) :
+let find_sample_cipher (#j:id) (#u:info) (s:sample) (#l:pne_plain_length) (c:pne_cipher l) (st:pne_state j u) (h:mem) :
   GTot bool =
   Some? (entry_for_sample_cipher s #l c st h)
 
 let sample_cipherpad_filter (j:id) (u:info) (s:sample) (cp:pne_cipherpad) (e:entry j u) : bool =
-  Entry?.s e = s && clip_cipherpad cp (Entry?.l e) = Entry?.c e
+  Entry?.s e `lbytes_eq` s && clip_cipherpad cp (Entry?.l e) `lbytes_eq` Entry?.c e
 
 let entry_for_sample_cipherpad (#j:id) (#u:info) (s:sample) (cp:pne_cipherpad) (st:pne_state j u) (h:mem) :
   GTot (option (entry j u)) =
@@ -107,25 +129,33 @@ let find_sample_cipherpad (#j:id) (#u:info) (s:sample) (cp:pne_cipherpad) (st:pn
 val create (j:id) (u:info) : ST (pne_state j u)
   (requires fun _ -> True)
   (ensures fun h0 st h1 ->
-    modifies_none h0 h1 /\
-    table st h1 == Seq.empty)
+    invariant st h1 /\
 
+    B.modifies B.loc_none h0 h1 /\
+    B.fresh_loc (footprint st) h0 h1 /\
+    B.(loc_includes (loc_pne_region ()) (footprint st)) /\
+
+    (I.ideal_PRF && I.is_pne_honest j ==> table st h1 == Seq.empty))
+
+// JP: how can I write a proper functional specification here? I need to:
+// - generate a block of padding
+// - take the pn_offset to know where to find the mask
+// - the pn_offset depends on the cidlen
+// - cidlen is not available
 val encrypt :
   (#j:id) ->
   (#u:info) ->
   (st:pne_state j u) ->
-  (#l:pne_plainlen) ->
+  (#l:pne_plain_length) ->
   (n:pne_plain u j l) ->
   (s:sample) ->
   ST (pne_cipher l)
   (requires fun h0 ->
     fresh_sample s st h0)
   (ensures fun h0 c h1 ->
-    M.modifies (footprint st) h0 h1 /\
+    B.modifies (footprint st) h0 h1 /\
     (is_safe j ==>
       table st h1 == Seq.snoc (table st h0) (Entry s #l n c)))
-
-#reset-options "--z3rlimit 50"
 
 val decrypt :
   (#j:id) ->
@@ -133,7 +163,7 @@ val decrypt :
   (st:pne_state j u) ->
   (cp:pne_cipherpad) ->
   (s:sample) ->
-  ST (l:pne_plainlen & pne_plain u j l)
+  ST (l:pne_plain_length & pne_plain u j l)
   (requires fun h0 -> True)
   (ensures fun h0 (|l, n|) h1 ->
     modifies_none h0 h1 /\
@@ -141,6 +171,6 @@ val decrypt :
      (match entry_for_sample s st h0 with
         | Some (Entry _ #l' n' c') ->
         (l = l' /\ n = n') <==>
-        (l = l' /\ c' = clip_cipherpad cp l))
+        (l = l' /\ c' `lbytes_eq` clip_cipherpad cp l))
     )
   )
