src/Model.Helpers.fst
@@ -1,0 +1,24 @@
+module Model.Helpers
+
+let lbytes (l:nat) = b:Seq.seq Lib.IntTypes.uint8 { Seq.length b = l }
+
+let rec lbytes_eq (x y: Seq.seq Lib.IntTypes.uint8): Tot (b:bool { b <==> x `Seq.equal` y }) (decreases (Seq.length x)) =
+  if Seq.length x = 0 && Seq.length y = 0 then
+    true
+  else if Seq.length x = 0 && Seq.length y <> 0 then
+    false
+  else if Seq.length x <> 0 && Seq.length y = 0 then
+    false
+  else
+    let hx = Seq.head x in
+    let hy = Seq.head y in
+    let tx = Seq.tail x in
+    let ty = Seq.tail y in
+    if Lib.RawIntTypes.u8_to_UInt8 hx = Lib.RawIntTypes.u8_to_UInt8 hy && lbytes_eq tx ty then begin
+      assert (x `Seq.equal` Seq.append (Seq.create 1 hx) tx);
+      assert (y `Seq.equal` Seq.append (Seq.create 1 hy) ty);
+      assert (Seq.index (Seq.create 1 hx) 0 == Seq.index (Seq.create 1 hy) 0);
+      assert (Seq.create 1 hx `Seq.equal` Seq.create 1 hy);
+      true
+    end else
+      false
